\subsection{Analysis}

\para{Fixed point.} We denote:

\begin{equation}
\begin{array}{l}
a(t) = 1 - {(1 - p(t))^{\tau {R_C}(t)}},b(t) = \frac{{p(t)}}{{{{(1 - p(t))}^{ - B}} - 1}},\\
c(t) = \frac{{{{(1 - p(t))}^{FB}}p(t)}}{{{{(1 - p(t))}^{ - B}} - 1}},d(t) = \frac{{p(t)}}{{{{(1 - p(t))}^{ - T{R_C}(t)}} - 1}},\\
e(t) = \frac{{{{(1 - p(t))}^{FT{R_C}(t)}}p(t)}}{{{{(1 - p(t))}^{ - T{R_C}(t)}} - 1}}
\end{array}
\end{equation}

DCQCN has a unique fixed point:

\begin{equation}
\small
{R_C^*} = \frac{C}{N}
\end{equation}
\begin{equation}
\small
\alpha^*  = 1 - {(1 - p)^{\frac{{\tau 'C}}{N}}}
\end{equation}
\begin{equation}
\small
{R_T^*} = \frac{C}{N} + \frac{{a\alpha }}{{(b + d)\tau }}
\end{equation}

\begin{equation}
\small
{q^*} = \frac{{{p^*}}}{{{p_{max}}}}\left( {{K_{max}} - {K_{min}}} \right) + {K_{min}}
\end{equation}

$p^*$ is determined by:
\begin{equation}
\small
\frac{{{a^2}\alpha }}{{(b + d)(c + e)}} = \frac{{{\tau ^2}{R_{AI}}C}}{N}
\end{equation}

We obtain the taylor series around $p=0$ of the left hand side:
\begin{equation}
\small
\frac{{{a^2}\alpha }}{{(b + d)(c + e)}} = \frac{{{C^3}{\tau ^2}\tau '}}{{{N^3}{{\left( {\frac{1}{B} + \frac{N}{{CT}}} \right)}^2}}}{p^3} + O\left( {{p^4}} \right)
\end{equation}

\begin{equation}
\small
{p^*} = \sqrt[3]{{\frac{{{R_{AI}}{N^2}}}{{\tau '{C^2}}}{{\left( {\frac{1}{B} + \frac{N}{{CT}}} \right)}^2}}}
\end{equation}

\para{Stability analysis.} 
We linearize the system by $\delta {R_C}(t) = {R_C}(t) - R_C^*$, $\delta {R_C}(t) = {R_C}(t) - R_C^*$,
$\delta p(t) = p(t) - p^*$, $\delta \alpha (t) = \alpha (t) - \alpha^*$, and $A = \left( {\frac{1}{B} + \frac{1}{{TR_C^*}}} \right)$.

\begin{equation}
\small
\begin{array}{l}
s{R_C}(s) - \delta {R_C}(0) = \left( { - \frac{1}{2}{{(R_C^*)}^2}{\alpha ^*} - \left( {\frac{1}{2} + \frac{A}{4}} \right)R_C^*R_T^* + \left( {\frac{1}{2} + \frac{A}{4}} \right){{(R_C^*)}^2}} \right){e^{ - s\tau *}}p(s)\\
 + \left( { - \frac{1}{2}{p^*}R_C^*{\alpha ^*} - \frac{A}{2}R_C^* + \left( {\frac{1}{2} + \frac{A}{4}} \right){p^*}R_C^*} \right){e^{ - s\tau *}}{R_C}(s)\\
 + \left( { - \frac{1}{2}{p^*}R_C^*{\alpha ^*} - \frac{A}{2}R_C^* + \frac{A}{2}R_T^* + \left( {\frac{1}{2} + \frac{A}{4}} \right){p^*}R_C^* - \left( {\frac{1}{2} + \frac{A}{4}} \right){p^*}R_T^*} \right){R_C}(s)\\
 - \frac{1}{2}{p^*}{(R_C^*)^2}\alpha (s)\\
 + \left( {\frac{A}{2}R_C^* - \left( {\frac{1}{2} + \frac{A}{4}} \right){p^*}R_C^*} \right){R_T}(s)
\end{array}
\end{equation}

\subsection{Convergence}
